Begin working on pointer permutation.

memory_safety/propertyA.v
@@ -3,7 +3,8 @@ Require Import Ssreflect.ssrnat Ssreflect.seq Ssreflect.eqtype Ssreflect.fintype
 
 Require Import MathComp.path MathComp.fingraph.
 
-Require Import CoqUtils.ord CoqUtils.word CoqUtils.partmap CoqUtils.fset.
+Require Import CoqUtils.ord CoqUtils.word CoqUtils.fset CoqUtils.partmap.
+Require Import CoqUtils.fperm.
 
 Require Import lib.utils lib.partmap_utils common.types.
 Require Import memory_safety.property memory_safety.abstract.
@@ -38,6 +39,8 @@ Implicit Type s : state.
 Implicit Type b : block.
 Implicit Type p : pointer.
 Implicit Type bs : {fset block}.
+Implicit Type v : value.
+Implicit Type pm : {fperm block}.
 
 Definition references m b b' :=
   [exists offs : mword mt * mword mt,
@@ -257,6 +260,38 @@ eapply ValidFree; simpl; first by eauto.
     by rewrite eq_b'' (free_get_fail hm').
   by rewrite (free_get hm') // eq_sym.
 by apply/hbs => {get_pc'}; eapply ReachBaseReg; eauto.
+Qed.
+
+Definition perm_ptr pm p := (pm p.1, p.2).
+
+Definition perm_value pm v :=
+  match v with
+  | VData w => VData block w
+  | VPtr p => VPtr (perm_ptr pm p)
+  end.
+
+Definition perm_regs pm rs := mapm (perm_value pm) rs.
+
+Definition perm_mem pm m :=
+  mkpartmapf (pm @: domm m)
+             (fun b => map (perm_value pm)
+                           (odflt [::] (m (fperm_inv pm b)))).
+
+Lemma perm_memP pm m p :
+  getv (perm_mem pm m) p =
+  omap (perm_value pm) (getv m (perm_ptr (fperm_inv pm) p)).
+Proof.
+case: p => [b o]; rewrite /getv mkpartmapfE /=.
+case: ifPn=> [b_def|b_ndef].
+  move/(mem_imfset (fperm_inv pm)): b_def.
+  rewrite -imfset_comp -(imfset_eq (fpermM _ pm)) fperm_mulKV.
+  rewrite (imfset_eq (@fperm1 _)) imfset_id=> /dommP [fr efr].
+  rewrite efr /= size_map.
+  have [lt|] //= := boolP (o < size fr).
+  by congr Some; apply: (nth_map _ _ _ lt).
+case b_def: (m _) => //.
+have/(mem_imfset pm) : fperm_inv pm b \in domm m by apply/dommP; eauto.
+by rewrite fpermKV; move=> h; rewrite h in b_ndef.
 Qed.
 
 End MemorySafety.
